Cslib/Foundations/Semantics/Algebra/Basic.lean
@@ -1,0 +1,146 @@
+/-
+Copyright (c) 2026 Thomas Waring. All rights reserved.
+Released under Apache 2.0 license as described in the file LICENSE.
+Authors: Thomas Waring
+-/
+
+module
+
+public import Cslib.Foundations.Syntax.Term.Basic
+public import Mathlib.Data.Setoid.Basic
+
+public section
+
+namespace Cslib
+
+universe u v
+
+class SAlgebra (S : Signature.{v}) (A : Type u) : Type (max (u + 1) (v + 1)) where
+  interp (f : S.Sym) : (Fin (S.arity f) → A) → A
+
+namespace SAlgebra
+
+variable {S : Signature} {A B C : Type u} [SAlgebra S A] [SAlgebra S B] [SAlgebra S C]
+
+structure SAlgHom (S : Signature) (A B : Type u) [iA : SAlgebra S A] [iB : SAlgebra S B] where
+  toFun : A → B
+  map_interp' {f : S.Sym} (xs : Fin (S.arity f) → A) : toFun (interp f xs) = interp f (toFun ∘ xs)
+
+scoped notation A " →[" S "] " B => SAlgHom S A B
+
+namespace SAlgHom
+
+variable {ψ : B →[S] C} {φ : A →[S] B}
+
+instance instFunLike : FunLike (A →[S] B) A B where
+  coe := SAlgHom.toFun
+  coe_injective' φ ψ h := by cases φ; cases ψ; grind
+
+@[simp]
+lemma map_interp (φ : A →[S] B) {f : S.Sym} (xs : Fin (S.arity f) → A) :
+    φ (interp f xs) = interp f (φ ∘ xs) := SAlgHom.map_interp' ..
+
+def id (A : Type u) [SAlgebra S A] : A →[S] A where
+  toFun x := x
+  map_interp' _ := rfl
+
+lemma id_apply (x : A) : @id S A _ x = x := by rfl
+
+def comp (ψ : B →[S] C) (φ : A →[S] B) : A →[S] C where
+  toFun := ψ ∘ φ
+  map_interp' xs := by simp [Function.comp_assoc]
+
+lemma comp_apply (x : A) : (ψ ∘ φ) x = ψ (φ x) := rfl
+
+-- comp_id, id_comp, etc etc
+
+end SAlgHom
+
+structure SAlgIso (S : Signature) (A B : Type u) [iA : SAlgebra S A] [iB : SAlgebra S B] where
+  toHom : A →[S] B
+  invHom : B →[S] A
+  left_inv : Function.LeftInverse invHom toHom
+  right_inv : Function.RightInverse invHom toHom
+
+scoped notation A " ≅[" S "] " B => SAlgIso S A B
+
+-- TODO composition, coercions etc for `SAlgIso`
+
+structure Congruence (S : Signature) (A : Type u) [SAlgebra S A] where
+  toRel : A → A → Prop
+  iseqv : Equivalence toRel
+  map_interp {f : S.Sym} {xs ys : Fin (S.arity f) → A} (hxs : ∀ i, toRel (xs i) (ys i)) :
+      toRel (interp f xs) (interp f ys)
+
+namespace Congruence
+
+protected def Setoid (r : Congruence S A) : Setoid A where
+  r := r.toRel
+  iseqv := r.iseqv
+
+lemma setoid_coe (r : Congruence S A) : (r.Setoid : A → A → Prop) = r.toRel := by
+  rw [Setoid.r, Congruence.Setoid]
+
+set_option quotPrecheck false in
+scoped notation:max A "⧸" r => Quotient (r : Congruence S A).Setoid
+
+/--
+It's possible to make this computable but only because the indexing type `Fin (S.arity f)` is a
+Fintype (see `Setoid.piQuotientEquiv`). It would involve some horrible fold though which I can't
+bring myself to code. The result `Congruence.quotient_interp_mk_eq` ensures this definition matches
+the "real" one.
+-/
+noncomputable instance instSAlgebraQuotient (r : Congruence S A) :
+    SAlgebra S A⧸r where
+  interp f ps := Quotient.mk'' (interp f <| fun i => (ps i).out)
+
+lemma interp_def {r : Congruence S A} {f : S.Sym} (ps : Fin (S.arity f) → A⧸r) :
+    interp f ps = ⟦interp f <| fun i => (ps i).out⟧ := rfl
+
+theorem quotient_mk_interp_eq (r : Congruence S A) {f : S.Sym} (xs : Fin (S.arity f) → A) :
+    Quotient.mk r.Setoid (interp f xs) =
+      interp (A := A⧸r) f (Quotient.mk r.Setoid ∘ xs) := by
+  symm
+  apply Quotient.sound
+  apply r.map_interp
+  simp_rw [←setoid_coe]
+  exact fun i => Quotient.mk_out' (xs i)
+
+def mk_hom (r : Congruence S A) : A →[S] (A⧸r) where
+  toFun := Quotient.mk r.Setoid
+  map_interp' := r.quotient_mk_interp_eq
+
+lemma mk_hom_surjective (r : Congruence S A) : Function.Surjective r.mk_hom :=
+  Quotient.mk_surjective
+
+def ofSAlgHom (φ : SAlgHom S A B) : Congruence S A where
+  toRel x y := φ x = φ y
+  iseqv := (Setoid.ker φ).iseqv
+  map_interp h := by
+    rw [φ.map_interp, φ.map_interp]
+    congr 1
+    ext i
+    exact h i
+
+protected def lift {r : Congruence S A} (φ : A →[S] B) (h : ∀ x y : A, r.toRel x y → φ x = φ y) :
+    (A⧸r) →[S] B where
+  toFun := Quotient.lift φ h
+  map_interp' xs := by
+    rw [r.interp_def, Quotient.lift_mk, φ.map_interp]
+    congr 1
+    ext i
+    rw [Function.comp_apply, Function.comp_apply, ←Quotient.out_eq (q := xs i), Quotient.lift_mk]
+    simp
+
+protected lemma lift_comp_mk {r : Congruence S A} (φ : A →[S] B)
+    (h : ∀ x y : A, r.toRel x y → φ x = φ y) : (r.lift φ h).comp r.mk_hom = φ :=
+  DFunLike.coe_injective' <| DFunLike.ext'_iff.mp rfl
+
+end Congruence
+
+-- might run into universe issues here?
+instance instPiSAlgebra {κ : Type _} (As : κ → Type _) [∀ k, SAlgebra S (As k)] :
+    SAlgebra S (Π k, As k) where
+  interp f xs k := interp f (fun i => xs i k)
+
+end Cslib.SAlgebra
